src/doc.sh
@@ -1,18 +1,12 @@
 #!/bin/sh
 
-# We cat files rather than passing them as args
-# to work around an apparent coqdoc notation printing bug whereby [1] fails.
-# [1] http://comments.gmane.org/gmane.science.mathematics.logic.coq.club/5894
-cat \
+coqdoc --short --light --body-only --latex -o body.tex \
   Notations.v \
   Codes.v \
-  IndexedCodes.v \
-  Points.v \
-  ObAxioms.v \
-  Lambda.v \
-  Bohm.v \
   Constructor.v \
   Types.v \
-| coqdoc --short --light --body-only --latex -o body.tex
+  IndexedCodes.v \
+  Points.v \
+  #
 
 pdflatex main.tex
